complete counter client

theories/coneris/examples/random_counter/client.v
@@ -35,35 +35,6 @@ Section lemmas.
   Qed.
 End lemmas.
 
-Section lemmas'.
-  Context `{!inG Σ (excl_authR (boolO))}.
-
-  (* Helpful lemmas *)
-  Lemma ghost_var_alloc' b :
-    ⊢ |==> ∃ γ, own γ (●E b) ∗ own γ (◯E b).
-  Proof.
-    iMod (own_alloc (●E b ⋅ ◯E b)) as (γ) "[??]".
-    - by apply excl_auth_valid.
-    - by eauto with iFrame.
-  Qed.
-
-  Lemma ghost_var_agree' γ b c :
-    own γ (●E b) -∗ own γ (◯E c) -∗ ⌜ b = c ⌝.
-  Proof.
-    iIntros "Hγ● Hγ◯".
-    by iCombine "Hγ● Hγ◯" gives %->%excl_auth_agree_L.
-  Qed.
-
-  Lemma ghost_var_update' γ b' b c :
-    own γ (●E b) -∗ own γ (◯E c) ==∗ own γ (●E b') ∗ own γ (◯E b').
-  Proof.
-    iIntros "Hγ● Hγ◯".
-    iMod (own_update_2 _ _ _ (●E b' ⋅ ◯E b') with "Hγ● Hγ◯") as "[$$]".
-    { by apply excl_auth_update. }
-    done.
-  Qed.
-End lemmas'.
-
 Section client.
   Context `{rc:random_counter} {L: counterG Σ}.
   Definition con_prog : expr :=
@@ -76,9 +47,34 @@ Section client.
     read_counter "c"
   .
 
-  Definition counter_nroot:=nroot.@"counter".
+  Definition one_positive n1 n2:=
+    match (n1, n2) with
+    | (Some (S _), _) | (_, Some (S _)) => true
+    | _ => false
+    end.
 
+  Definition counter_nroot:=nroot.@"counter".
+  Definition inv_nroot:=nroot.@"inv".
+  
   Context `{!spawnG Σ, !inG Σ (excl_authR (option natO)), !inG Σ (excl_authR (boolO))}.
+
+  Definition con_prog_inv (γ1 γ2: gname): iProp Σ :=
+    ∃ (n1 n2 : option nat) ,
+      let p:= one_positive n1 n2 in
+      own γ1 (●E n1) ∗ own γ2 (●E n2) ∗
+      if p
+      then ↯ 0%R
+      else
+        ∃ (flip_num:nat),
+          ↯ (Rpower 4%R (INR flip_num-2))%R ∗
+          ⌜(flip_num = bool_to_nat (bool_decide (n1=Some 0%nat)) +bool_to_nat (bool_decide (n2=Some 0%nat)))%nat⌝.
+
+  Lemma Rpower_4_2: (Rpower 4 2 = 16)%R.
+  Proof.
+    replace 2%R with (1+1)%R by lra.
+    rewrite Rpower_plus Rpower_1; lra.
+  Qed.
+  
   Lemma con_prog_spec:
     {{{ ↯ (1/16) }}}
       con_prog
@@ -86,12 +82,137 @@ Section client.
   Proof.
     iIntros (Φ) "Hε HΦ".
     rewrite /con_prog.
-    wp_apply (new_counter_spec _ counter_nroot with "[//]") as (c) "(%γ & #Hcounter & Hfrag)".
+    wp_apply (new_counter_spec (L:=L) _ counter_nroot with "[//]") as (c) "(%γ & #Hcounter & Hfrag)".
     replace (1)%Qp with (1/2+1/2)%Qp; last compute_done.
     replace 0%nat with (0+0)%nat by lia.
-    rewrite -counter_content_frag_combine.
-    iDestruct "Hfrag" as "[Hfrag1 Hfrag2]".
+    rewrite -(counter_content_frag_combine).
+    iDestruct "Hfrag" as "[Hc1 Hc2]".
     wp_pures.
-  Admitted.
+    iMod (ghost_var_alloc None) as (γ1) "[Hauth1 Hfrag1]".
+    iMod (ghost_var_alloc None) as (γ2) "[Hauth2 Hfrag2]".
+    iMod (inv_alloc inv_nroot _ (con_prog_inv γ1 γ2) with "[Hauth1 Hauth2 Hε]") as "#Hinv".
+    { iModIntro. iFrame. iExists _. iSplit; last done.
+      simpl. replace (0-2)%R with (-2)%R by lra.
+      rewrite Rpower_Ropp Rpower_4_2.
+      iApply (ec_eq with "[$]").
+      lra.
+    }
+    wp_apply (wp_par (λ _, ∃ (n:nat), own γ1 (◯E (Some n)) ∗ counter_content_frag γ (1/2) n)%I
+                (λ _, ∃ (n:nat), own γ2 (◯E (Some n)) ∗ counter_content_frag γ (1/2) n)%I with "[Hfrag1 Hc1][Hfrag2 Hc2]").
+    - wp_apply (allocate_tape_spec with "[$]") as (lbl) "Htape"; first done.
+      wp_pures.
+      iAssert (state_update ⊤ ⊤ (∃ n, own γ1 (◯E (Some n)) ∗ counter_tapes lbl [n]))%I with "[Hfrag1 Htape]" as ">(%n & Hfrag1 & Htape)".
+      { iApply (state_update_inv_acc with "[$]"); first done.
+        iIntros ">(%n1 & %n2 & Hauth1 & Hauth2 & Herr)".
+        iDestruct (ghost_var_agree with "[$Hauth1][$]") as "->".
+        case_match eqn:H.
+        - iMod (counter_tapes_presample _ _ _ _ _ _ _ (λ _, 0%R) with "[$][$][$]") as "(%n & Herr & Htape)".
+          + apply namespaces.coPset_subseteq_difference_r; last done.
+            by apply ndot_ne_disjoint.
+          + done.
+          + rewrite SeriesC_0; intros; lra.
+          + iMod (ghost_var_update _ (Some (fin_to_nat n)) with "[$Hauth1][$]") as "[Hauth1 Hfrag1]".
+            simpl. iFrame.
+            iModIntro.
+            case_match; first done.
+            destruct n as [|]; destruct n2 as [[]|]; simplify_eq.
+        - iDestruct "Herr" as "(%&Herr&->)/=".
+          iMod (counter_tapes_presample _ _ _ _ _ _ _ (λ x, if 0<? fin_to_nat x then 0%R else (Rpower 4 (1+(bool_to_nat (bool_decide (n2 = Some 0%nat)) - 2))))%R with "[$][$][$]") as "(%n & Herr & Htape)".
+          + apply namespaces.coPset_subseteq_difference_r; last done.
+            by apply ndot_ne_disjoint.
+          + intros. case_match; first done. rewrite /Rpower. left. apply exp_pos.
+          + rewrite SeriesC_finite_foldr/=.
+            rewrite Rpower_plus Rpower_1; lra.
+          + iMod (ghost_var_update _ (Some (fin_to_nat n)) with "[$Hauth1][$]") as "[Hauth1 Hfrag1]".
+            simpl. iFrame.
+            iModIntro.
+            case_match eqn:H0.
+            * case_match; first done.
+              destruct (fin_to_nat n) as [|]; destruct n2 as [[|]|]; simplify_eq.
+            * case_match.
+              { destruct (fin_to_nat n) as [|]; destruct n2 as [[|]|]; simplify_eq. }
+              iExists _. iSplit; last done.
+              iApply (ec_eq with "[$]").
+              f_equal.
+              rewrite plus_INR. 
+              assert (fin_to_nat n = 0)%nat as ->; simpl; last lra.
+              apply Z.ltb_ge in H0. lia.
+      }
+      wp_apply (incr_counter_tape_spec_some _ _ _ _ (λ _, counter_content_frag γ (1/2) n)%I with "[$Htape $Hcounter Hc1]"); first done.
+      { iIntros (?) "?".
+        iMod (counter_content_update with "[$][$]") as "[$ ?]".
+        by simpl.
+      }
+      iIntros (?) "[??]". iFrame.
+    - wp_apply (allocate_tape_spec with "[$]") as (lbl) "Htape"; first done.
+      wp_pures.
+      iAssert (state_update ⊤ ⊤ (∃ n, own γ2 (◯E (Some n)) ∗ counter_tapes lbl [n]))%I with "[Hfrag2 Htape]" as ">(%n & Hfrag2 & Htape)".
+      { iApply (state_update_inv_acc with "[$]"); first done.
+        iIntros ">(%n1 & %n2 & Hauth1 & Hauth2 & Herr)".
+        iDestruct (ghost_var_agree with "[$Hauth2][$]") as "->".
+        case_match eqn:H.
+        - iMod (counter_tapes_presample _ _ _ _ _ _ _ (λ _, 0%R) with "[$][$][$]") as "(%n & Herr & Htape)".
+          + apply namespaces.coPset_subseteq_difference_r; last done.
+            by apply ndot_ne_disjoint.
+          + done.
+          + rewrite SeriesC_0; intros; lra.
+          + iMod (ghost_var_update _ (Some (fin_to_nat n)) with "[$Hauth2][$]") as "[Hauth2 Hfrag2]".
+            simpl. iFrame.
+            iModIntro.
+            case_match; first done.
+            destruct n as [|]; destruct n1 as [[]|]; simplify_eq.
+        - iDestruct "Herr" as "(%&Herr&->)/=".
+          iMod (counter_tapes_presample _ _ _ _ _ _ _ (λ x, if 0<? fin_to_nat x then 0%R else (Rpower 4 (1+((bool_to_nat (bool_decide (n1 = Some 0)) + 0)%nat - 2))))%R with "[$][$][$]") as "(%n & Herr & Htape)".
+          + apply namespaces.coPset_subseteq_difference_r; last done.
+            by apply ndot_ne_disjoint.
+          + intros. case_match; first done. rewrite /Rpower. left. apply exp_pos.
+          + rewrite SeriesC_finite_foldr/=.
+            rewrite Rpower_plus Rpower_1; lra.
+          + iMod (ghost_var_update _ (Some (fin_to_nat n)) with "[$Hauth2][$]") as "[Hauth2 Hfrag2]".
+            simpl. iFrame.
+            iModIntro.
+            case_match eqn:H0.
+            * case_match; first done.
+              destruct (fin_to_nat n) as [|]; destruct n1 as [[|]|]; simplify_eq.
+            * case_match.
+              { destruct (fin_to_nat n) as [|]; destruct n1 as [[|]|]; simplify_eq. }
+              iExists _. iSplit; last done.
+              iApply (ec_eq with "[$]").
+              f_equal.
+              rewrite !plus_INR. 
+              assert (fin_to_nat n = 0)%nat as ->; simpl; last lra.
+              apply Z.ltb_ge in H0. lia.
+      }
+      wp_apply (incr_counter_tape_spec_some _ _ _ _ (λ _, counter_content_frag γ (1/2) n)%I with "[$Htape $Hcounter Hc2]"); first done.
+      { iIntros (?) "?".
+        iMod (counter_content_update with "[$][$]") as "[$ ?]".
+        by simpl.
+      }
+      iIntros (?) "[??]". iFrame.
+    - iIntros (??) "[(%n1 & Hfrag1 & Hc1)(%n2 & Hfrag2 & Hc2)]".
+      iNext. wp_pures.
+      iCombine "Hc1 Hc2" as "Hc".
+      rewrite counter_content_frag_combine.
+      replace (1/2+1/2)%Qp with 1%Qp; last compute_done.
+      iAssert (|={⊤}=> ⌜(n1+n2>0)%nat⌝)%I with "[Hfrag1 Hfrag2]" as ">%".
+      { iInv "Hinv" as ">(%&%&Hauth1&Hauth2&Herr)".
+        iDestruct (ghost_var_agree with "[$Hauth1][$]") as "->".
+        iDestruct (ghost_var_agree with "[$Hauth2][$]") as "->".
+        rewrite /con_prog_inv.
+        destruct n1, n2 as [|]; [simpl|simpl; iModIntro; iFrame; iSplitL "Herr"; iModIntro; try (iPureIntro; lia); done..]; last first.
+        iDestruct "Herr" as "(%&Herr&->)".
+        simpl. replace (_+_-_)%R with 0%R by lra.
+        rewrite Rpower_O; last lra.
+        by iDestruct (ec_contradict with "[$]") as "[]".
+      }
+      wp_apply (read_counter_spec _ _ _ _ (λ n, ⌜(n>0)%nat⌝)%I with "[$Hcounter Hc]"); first done.
+      { iIntros.
+        iDestruct (counter_content_agree with "[$][$]") as "<-".
+        iFrame. iModIntro. iPureIntro. lia.
+      }
+      iIntros.
+      iApply "HΦ".
+      iPureIntro; lia.
+  Qed.
   
 End client.
